\documentclass{ximera}
\usepackage{tikz}
\begin{document}
\subsection{Differentiation Rules}
\begin{dialogue}
\item[Julia] Hmm...I don't think differentiation rules, it takes so long and I hate using that long limit definition!
\item[Dylan] No no Julia, it's differentiation \textit{rules}!
\item[Julia] Ohhhh, that makes more sense!

\end{dialogue}
\subsubsection{The Power Rule}
\begin{dialogue}
\item[Julia] I hate how long it takes to differentiate powers!
\item[Dylan] Yeah, it takes forever! I feel like there was some sort of pattern to it though. I couldn't figure anything out though.
\item[James] Sounds like you guys need my help again?
\item[Julia and Dylan] Help us James!
\item[James] There \textit{is} a pattern! Check out this table I made!
\begin{center}
\begin{tabular}{c|c}
$f(x)$ & $f'(x)$ \\
\hline
$x^2$ & $2x^1$ \\
$x^3$ & $3x^2$ \\
$x^4$ & $4x^3$ 
\end{tabular}
\end{center}
\end{dialogue}
\begin{question}
What pattern do you notice in James' table?
\begin{freeResponse}
This is the model solution %You don’t actually need anything in between the begin and end line.
\end{freeResponse}
\end{question}
\begin{question}
Generalize this pattern in terms of $x^n$

$ \frac{\partial}{\partial x} x^n =  \answer{n*x^(n-1)}$
\end{question}

\begin{question}
Using the limit definition of a derivative, compute the derivative for $x^5$

$ \frac{\partial}{\partial x} x^5 =  \answer{5x^4}$
\end{question}

\subsubsection{The Constant Rule}
\begin{dialogue}
\item[Dylan] Wow! That's neat!
\item[Julia] I wish we could use rules like this all over the place though, it would really save me time.
\item[James] There are plenty of places with rules like this! Why don't we look at a function like $y = 3$?
\end{dialogue}

Consider $y = c$, where $c$ is some arbitrary constant.
\begin{question}
Derive this function using the limit definition. What does your answer mean?

$ \frac{\partial y}{\partial x} (y=c) =  \answer{0}$
\begin{freeResponse}
This is the model solution %You don’t actually need anything in between the begin and end line.
\end{freeResponse}
\end{question}

\begin{question}
Using what you found in the previous problem, compute the following derivatives:

$ \frac{\partial}{\partial x=2}(y=c) =  \answer{0}$
$ \frac{\partial}{\partial x=100}(y=c) =  \answer{0}$
$ \frac{\partial}{\partial x=0}(y=c) =  \answer{0}$
\end{question}

\subsubsection{The Constant Multiple Rule}
\begin{dialogue}
\item[Julia] James! Show us more! These things are going to save me so much time on my homework!
\item[James] Alright alright, calm down Julia. We can look at a function like $y = 3x$ next.
\end{dialogue}

Consider $y = kx$, where $k$ is some arbitrary constant.
\begin{question}
$ \frac{\partial y}{\partial x} (k*x) =  \answer{k}$
\item{What does your answer mean?}
\begin{freeResponse}
This is the model solution %You don’t actually need anything in between the begin and end line.
\end{freeResponse}
\end{question}

\begin{question}
\item{Using what you found in the previous problem, compute the following derivatives:}

$ \frac{\partial y}{\partial x} (4*x) =  \answer{4}$
$ \frac{\partial y}{\partial x} (10*x) =  \answer{10}$
$ \frac{\partial y}{\partial x} (\frac{1}{5}*x) =  \answer{\frac{1}{5}}$
\end{question}

\subsubsection{The Sum and Difference Rules}
\begin{dialogue}
\item[Dylan] Wow, this stuff is awesome! Is there any way to put it all together? Like, is there an easy way to tell what the derivative of $f(x) = 3x+4$ is?
\item[James] There is Dylan!
\end{dialogue}
Consider the differentiable functions $f(x)$ and $g(x)$. We will define a function $j(x) = f(x) + g(x)$.

\begin{enumerate}
\item{Take the derivative of $j(x)$ using the limit definition. What does your answer mean? \textit{Hint: In $j(x+h)$, the $(x+h)$ will replace $x$ in the component functions as well.}}

$ j'(x) =  \answer{\frac{\j(x+h)-j(x)}{h}}$
\item{Using what you found in the previous problem, compute the following derivatives:
\item{$f(x) = 3x^2 - 5x + 2$, $g(x) = x^2 + 3x$}

$ j'(x) =  \answer{8x-2}$
\item{$f(x) = x^2 - 4x + 2$, $g(x) = -4x^2 + 3$}

$ j'(x) =  \answer{-6x-4}$
\item{$f(x) = 5x^3 + 3x$, $g(x) = 2x^2 - 13x$}

$ j'(x) =  \answer{15x^2+4x-10}$


\item{Julia wonders if a similar rule exists for $j(x) = f(x)-g(x)$. Using the limit definition of derivative, determine if there is a pattern. Then, if there is a rule, use it to solve the 1a, 1b, and 1c. If there is not, do them using the limit definition.}
\item{$f(x) = 3x^2 - 5x + 2$, $g(x) = x^2 + 3x$}

$ j'(x) =  \answer{4x-8}$
\item{$f(x) = x^2 - 4x + 2$, $g(x) = -4x^2 + 3$}

$ j'(x) =  \answer{-10x-4}$
\item{$f(x) = 5x^3 + 3x$, $g(x) = 2x^2 - 13x$}

$ j'(x) =  \answer{15x^2-4x+16}$
\end{enumerate}
\subsubsection{In Summary}
We've covered a lot of differentiation rules in this lab, to help you out we've made the following table.
\begin{center}
{\renewcommand{\arraystretch}{3}
\begin{tabular}{| l | p{7.5cm} |}
    \hline
    Power Rule & $\displaystyle \dfrac{d}{dx}(x^n)=n*x^{(n-1)}$,where $n$ is any real number besides 0. \\
    \hline
    Constant Rule & $\displaystyle\dfrac{d}{dx}(c) = 0$ \\
    \hline
    Constant Multiple Rule & $\displaystyle\dfrac{d}{dx}(cf(x))=c\dfrac{d}{dx}f(x)$ \\
    \hline
    Sum Rule & $\displaystyle\dfrac{d}{dx}(f(x)+g(x))=\dfrac{d}{dx}f(x)+\dfrac{d}{dx}g(x)$ \\
    \hline
    Difference Rule & $\displaystyle\dfrac{d}{dx}(f(x)-g(x))=\dfrac{d}{dx}f(x)-\dfrac{d}{dx}g(x)$ \\
    \hline
\end{tabular}}
\end{center}
\pagebreak
\end{document}